src/extensions/paths/Lookup.v
@@ -21,37 +21,37 @@ Inductive lookup_step : sta -> def_rhs -> def_rhs -> Prop :=
 (** [s(x) = v ]   #<br>#
     [―――――――――]   #<br>#
     [s[x ⤳ v]]   *)
-| lookup_var : forall s x v,
-    binds x v s ->
-    s ⟦ pvar x ⤳ defv v ⟧
+| lookup_var : forall γ x v,
+    binds x v γ ->
+    γ ⟦ pvar x ⤳ defv v ⟧
 
 (** [s ⟦ p ⤳ q ⟧ ]              #<br>#
     [――――――――――――――――――――――]    #<br>#
     [s ⟦ p.a ⤳ q.a ⟧ ]          *)
-| lookup_sel_p : forall s p q a,
-    s ⟦ p ⤳ defp q ⟧ ->
-    s ⟦ p•a ⤳ defp (q•a) ⟧
+| lookup_sel_p : forall γ p q a,
+    γ ⟦ p ⤳ defp q ⟧ ->
+    γ ⟦ p•a ⤳ defp (q•a) ⟧
 
 (** [s ⟦ p ⤳ ν(T)...{a = t}... ⟧ ]   #<br>#
     [――――――――――――――――――――――]         #<br>#
     [s ⟦ p.a ⤳ t ⟧ ]                 *)
-| lookup_sel_v : forall s p a t T ds,
-    s ⟦ p ⤳ defv (val_new T ds) ⟧ ->
+| lookup_sel_v : forall γ p a t T ds,
+    γ ⟦ p ⤳ defv (val_new T ds) ⟧ ->
     defs_has ds { a := t } ->
-    s ⟦ p•a ⤳ open_defrhs_p p t ⟧
+    γ ⟦ p•a ⤳ open_defrhs_p p t ⟧
 
-where "s '⟦' p '⤳' t '⟧'" := (lookup_step s (defp p) t).
+where "γ '⟦' p '⤳' t '⟧'" := (lookup_step γ (defp p) t).
 
 (** Reflexive, transitive closure of path lookup *)
-Notation "s '⟦' t '⤳*' u '⟧'" := (star (lookup_step s) t u) (at level 40).
+Notation "γ '⟦' t '⤳*' u '⟧'" := (star (lookup_step γ) t u) (at level 40).
 
 (** Path lookup that results in values *)
 Inductive lookup : sta -> path * val -> Prop :=
-| lookup_def: forall s p v,
-    s ⟦ defp p ⤳* defv v ⟧ ->
-    s ∋ (p, v)
+| lookup_def: forall γ p v,
+    γ ⟦ defp p ⤳* defv v ⟧ ->
+    γ ∋ (p, v)
 
-where "s '∋' t" := (lookup s t).
+where "γ '∋' t" := (lookup γ t).
 
 Hint Constructors lookup lookup_step.
 
@@ -69,19 +69,19 @@ Ltac solve_lookup :=
     rewrite <- H; econstructor; simpl_dot; eauto
   end.
 
-Lemma lookup_strengthen_one: forall s y v x bs t,
-    s & y ~ v ⟦ p_sel (avar_f x) bs ⤳ t ⟧ ->
+Lemma lookup_strengthen_one: forall γ y v x bs t,
+    γ & y ~ v ⟦ p_sel (avar_f x) bs ⤳ t ⟧ ->
     y <> x ->
-    s ⟦ p_sel (avar_f x) bs ⤳ t ⟧.
+    γ ⟦ p_sel (avar_f x) bs ⤳ t ⟧.
 Proof.
   introv Hl Hn. dependent induction Hl; try solve_lookup.
   constructor. eapply binds_push_neq_inv; eauto.
 Qed.
 
-Lemma lookup_strengthen s s1 s2 x v bs t :
-  ok s ->
-  s = s1 & x ~ v & s2 ->
-  s ⟦ p_sel (avar_f x) bs ⤳ t ⟧ ->
+Lemma lookup_strengthen γ s1 s2 x v bs t :
+  ok γ ->
+  γ = s1 & x ~ v & s2 ->
+  γ ⟦ p_sel (avar_f x) bs ⤳ t ⟧ ->
   s1 & x ~ v ⟦ p_sel (avar_f x) bs ⤳ t ⟧.
 Proof.
   intros Hok -> Hs. induction s2 using env_ind.
@@ -92,8 +92,8 @@ Proof.
       apply lookup_strengthen_one in Hs; auto.
 Qed.
 
-Lemma named_lookup_step: forall s t p,
-    s ⟦ p ⤳ t ⟧ ->
+Lemma named_lookup_step: forall γ t p,
+    γ ⟦ p ⤳ t ⟧ ->
     exists x bs, p = p_sel (avar_f x) bs.
 Proof.
   intros. dependent induction H.
@@ -102,16 +102,16 @@ Proof.
   - specialize (IHlookup_step _ eq_refl) as [? [? ->]]. simpl. repeat eexists; eauto.
 Qed.
 
-Lemma lookup_val_inv: forall s v t,
-    s ⟦ defv v ⤳* t ⟧ ->
+Lemma lookup_val_inv: forall γ v t,
+    γ ⟦ defv v ⤳* t ⟧ ->
     t = defv v.
 Proof.
   introv Hs. dependent induction Hs. auto. inversion H.
 Qed.
 
-Lemma lookup_step_func: forall s t t1 t2,
-    s ⟦ t ⤳ t1 ⟧ ->
-    s ⟦ t ⤳ t2 ⟧ ->
+Lemma lookup_step_func: forall γ t t1 t2,
+    γ ⟦ t ⤳ t1 ⟧ ->
+    γ ⟦ t ⤳ t2 ⟧ ->
     t1 = t2.
 Proof.
   introv Hl1. gen t2. dependent induction Hl1; introv Hl2.
@@ -123,52 +123,52 @@ Proof.
     lets Hd: (defs_has_inv H H0). subst*.
 Qed.
 
-Lemma lookup_irred: forall s v,
-    irred (lookup_step s) (defv v).
+Lemma lookup_irred: forall γ v,
+    irred (lookup_step γ) (defv v).
 Proof.
   inversion 1.
 Qed.
 
-Lemma lookup_func : forall s p v1 v2,
-    s ∋ (p, v1) ->
-    s ∋ (p, v2) ->
+Lemma lookup_func : forall γ p v1 v2,
+    γ ∋ (p, v1) ->
+    γ ∋ (p, v2) ->
     v1 = v2.
 Proof.
   introv Hs1 Hs2.
-  lets H: (lookup_step_func). specialize (H s). inversions Hs1. inversions Hs2.
-  assert (irred (lookup_step s) (defv v1)) as Hirr1 by apply* lookup_irred.
-  assert (irred (lookup_step s) (defv v2)) as Hirr2 by apply* lookup_irred.
-  assert (forall a b c : def_rhs, lookup_step s a b -> lookup_step s a c -> b = c) as H'. {
+  lets H: (lookup_step_func). specialize (H γ). inversions Hs1. inversions Hs2.
+  assert (irred (lookup_step γ) (defv v1)) as Hirr1 by apply* lookup_irred.
+  assert (irred (lookup_step γ) (defv v2)) as Hirr2 by apply* lookup_irred.
+  assert (forall a b c : def_rhs, lookup_step γ a b -> lookup_step γ a c -> b = c) as H'. {
     intros. destruct a; try solve [inversion H0]. apply* H.
   }
   lets Hf: (finseq_unique H' H2 Hirr1 H3 Hirr2). inversion* Hf.
 Qed.
 
-Lemma lookup_step_weaken_one : forall s x bs v y t,
-    s ⟦ p_sel (avar_f x) bs ⤳ t ⟧ ->
-    y # s ->
-    s & y ~ v ⟦ p_sel (avar_f x) bs ⤳ t ⟧.
+Lemma lookup_step_weaken_one : forall γ x bs v y t,
+    γ ⟦ p_sel (avar_f x) bs ⤳ t ⟧ ->
+    y # γ ->
+    γ & y ~ v ⟦ p_sel (avar_f x) bs ⤳ t ⟧.
 Proof.
   introv Hp Hn. dependent induction Hp; try solve_lookup.
   constructor. apply* binds_push_neq. intro. subst. eapply binds_fresh_inv; eauto.
 Qed.
 
-Lemma lookup_step_weaken s p t s' :
-  ok (s & s') ->
-  s ⟦ p ⤳ t ⟧ ->
-  s & s' ⟦ p ⤳ t ⟧.
+Lemma lookup_step_weaken γ p t γ' :
+  ok (γ & γ') ->
+  γ ⟦ p ⤳ t ⟧ ->
+  γ & γ' ⟦ p ⤳ t ⟧.
 Proof.
-  intros Hok Hs. induction s' using env_ind.
+  intros Hok Hs. induction γ' using env_ind.
   - rewrite concat_empty_r in *; auto.
   - rewrite concat_assoc in *. apply ok_push_inv in Hok as [Hok Hn].
     destruct (named_lookup_step Hs) as [y [bs ->]].
     apply* lookup_step_weaken_one.
 Qed.
 
-Lemma lookup_weaken_one : forall s x bs v y t,
-    s ⟦ defp (p_sel (avar_f x) bs) ⤳* t ⟧ ->
-    y # s ->
-    s & y ~ v ⟦ defp (p_sel (avar_f x) bs) ⤳* t ⟧.
+Lemma lookup_weaken_one : forall γ x bs v y t,
+    γ ⟦ defp (p_sel (avar_f x) bs) ⤳* t ⟧ ->
+    y # γ ->
+    γ & y ~ v ⟦ defp (p_sel (avar_f x) bs) ⤳* t ⟧.
 Proof.
   introv Hl Hn. gen y. dependent induction Hl; introv Hn.
   - apply star_refl.
@@ -181,12 +181,12 @@ Proof.
     * apply lookup_val_inv in Hl. subst. apply star_one. apply* lookup_step_weaken_one.
 Qed.
 
-Lemma lookup_weaken s t1 t2 s' :
-  ok (s & s') ->
-  s ⟦ t1 ⤳* t2 ⟧ ->
-  s & s' ⟦ t1 ⤳* t2 ⟧.
+Lemma lookup_weaken γ t1 t2 γ' :
+  ok (γ & γ') ->
+  γ ⟦ t1 ⤳* t2 ⟧ ->
+  γ & γ' ⟦ t1 ⤳* t2 ⟧.
 Proof.
-  intros Hok Hs. induction s' using env_ind.
+  intros Hok Hs. induction γ' using env_ind.
   - rewrite concat_empty_r in *; auto.
   - rewrite concat_assoc in *. apply ok_push_inv in Hok as [Hok Hn].
     assert (t1 = t2 \/ exists y bs, t1 = defp (p_sel (avar_f y) bs)) as [-> | [y [bs ->]]].
