src/extensions/paths/OperationalSemantics.v
@@ -10,28 +10,28 @@ Reserved Notation "t1 '⟼' t2" (at level 40, t2 at level 39).
 
 Inductive red : sta * trm -> sta * trm -> Prop :=
 
-(** [s ∋ (p, lambda(T)t)  ]      #<br>#
+(** [γ ∋ (p, lambda(T)t)  ]      #<br>#
     [―――――――――――――――――――――]      #<br>#
-    [(s, p q) ⟼ (s, t^q)]      *)
-| red_app: forall s p q T t,
-    s ∋ (p, λ(T) t) ->
-    (s, trm_app p q) ⟼ (s, open_trm_p q t)
+    [(γ p q) ⟼ (γ, t^q)]      *)
+| red_app: forall γ p q T t,
+    γ ∋ (p, λ(T) t) ->
+    (γ, trm_app p q) ⟼ (γ, open_trm_p q t)
 
-(** [(s, let x = v in t) ⟼ ((s, x = v), t^x)] *)
-| red_let_val : forall v t s x,
-    x # s ->
-    (s, trm_let (trm_val v) t) ⟼ (s & x ~ v, open_trm x t)
+(** [(γ, let x = v in t) ⟼ ((γ, x = v), t^x)] *)
+| red_let_val : forall v t γ x,
+    x # γ ->
+    (γ, trm_let (trm_val v) t) ⟼ (γ & x ~ v, open_trm x t)
 
-(** [(s, let y = p in t) ⟼ (s, t^p)] *)
-| red_let_path : forall t s p,
-    (s, trm_let (trm_path p) t) ⟼ (s, open_trm_p p t)
+(** [(γ, let y = p in t) ⟼ (γ, t^p)] *)
+| red_let_path : forall t γ p,
+    (γ, trm_let (trm_path p) t) ⟼ (γ, open_trm_p p t)
 
-(** [(s, t0) ⟼ (s', t0')]                            #<br>#
+(** [(γ, t0) ⟼ (γ', t0')]                            #<br>#
     [―――――――――――――――――――――――――――――――――――――――――――――――]  #<br>#
-    [(s, let x = t0 in t) ⟼ (s', let x = t0' in t)]  *)
-| red_let_tgt : forall t0 t s t0' s',
-    (s, t0) ⟼ (s', t0') ->
-    (s, trm_let t0 t) ⟼ (s', trm_let t0' t)
+    [(γ, let x = t0 in t) ⟼ (γ', let x = t0' in t)]  *)
+| red_let_tgt : forall t0 t γ t0' γ',
+    (γ, t0) ⟼ (γ', t0') ->
+    (γ, trm_let t0 t) ⟼ (γ', trm_let t0' t)
 
 where "t1 '⟼' t2" := (red t1 t2).
 
